---
author: Local Ghost
title: 'Linear Flow on the Torus'
tags: Math Topology Torus
categories: Math
---

**Theorem 1.1.**{:#theorem-linear-flow} 
Let $$\mathbb T^{n}=\mathbb R^{n}/ \mathbb Z^{n}$$ be a $$n$$-torus, $$\alpha_{i} \in \mathbb R, 1\leq i\leq n$$. Suppose $$r=\operatorname{dim}_{\mathbb Q} \sum \alpha_{i}\mathbb Q$$, then
the closure $$E$$ of $$t(\alpha_{i}), t \in \mathbb R$$ in $$\mathbb T^{n}$$ forms a $$(r-1)$$-subtorus of $$\mathbb T^{n}$$. Furthermore, if $$\alpha_{i_1}, \cdots, \alpha_{i_{r}}$$ is a maximal $$\mathbb Q$$-linearly independent subset of $$\alpha_{i}$$, and $$(\alpha_{i})=(\alpha_{i_{j}})A$$, then $$E=\prod _{i=1}^{n}\mathbb T_{i} \cdot A$$, where $$T_{i}=\mathbb T$$ if $$i$$ in $$i_{j}$$, and $$0$$ otherwise.

**Proof.**
We may reduce it to the case when $$r=n$$. For any $$\beta \in \mathbb R$$, let $$F_{\beta}=\left\{t(\alpha_{2}, \cdots, \alpha_{n}): t \alpha_1=\beta\right\}$$, then $$F_{\beta}=F_{0}+\frac{\beta}{\alpha_1}(\alpha_2, \cdots, \alpha_{n})$$. By [Theorem 1.2](#theorem-irrational-lattice), $$\operatorname{cl}F_0=\mathbb T^{n-1}$$, thus
\\[
E=\operatorname{cl}\bigcup (\beta, F_{\beta})\supset \bigcup \operatorname{cl}(\beta, F_{\beta})=\mathbb T \times \mathbb T^{n-1}=\mathbb T^{n}
\\]

**Theorem 1.2.**{:#theorem-irrational-lattice} 
Let $$1, \alpha_{i}, 1\leq i\leq n$$ be $$\mathbb Q$$-linear independent, then $$k(\alpha_{i}), k \in \mathbb Z$$ is dense in $$\mathbb T^{n}$$.

**Proof.**
We prove the statement by induction on $$n$$.
1.	if $$n=1$$, we show that any $$\beta \in \mathbb T$$ is a limit point of $$k \alpha$$: for any $$N \in \mathbb Z_{>0}$$, by [Pigeonhole Principle](https://en.wikipedia.org/wiki/Pigeonhole_principle), $$\exists 0<k<l\leq N+1$$ *s.t.* $$d(k \alpha, l \alpha)<\frac{1}{N}$$ for some $$t$$, thus $$k \alpha \in (-\frac{1}{N}, \frac{1}{N})$$ for some $$k \in \mathbb Z$$. Hence $$\exists k \in \mathbb Z: k \alpha-\beta \in (0, \frac{1}{N})$$.
2.	if $$n>1$$, let $$E_{N}=\operatorname{cl}\left\{k \alpha_{n}: k \alpha _{i}\in (-\frac{1}{N}, \frac{1}{N}), 1\leq i\leq n-1\right\}$$. It suffices to show that $$E_{N}=\mathbb T$$ for all $$N \in \mathbb Z_{>0}$$.
	If not, note that $$E_{N}\supseteq E_{N^{\prime}}$$ for $$N^{\prime}\geq N$$, and by induction hypothesis, $$E_{N}\neq \varnothing$$ for all $$N \in \mathbb Z_{>0}$$.
	Let $$E=\bigcap E_{N}\neq \varnothing$$, then $$E$$ is a closed proper subgroup of $$\mathbb T$$, thus $$E$$ is cyclic of order $$m \in \mathbb Z_{>0}$$, and $$\frac{1}{m}$$ is a generator of $$E$$.
	Replace $$\alpha_{n}$$ by $$m \alpha_{n}$$, we may assume that $$E=0$$, and $$\lim _{N \to \infty}r(E_{N})\to 0$$.
	Pick a suitable $$N$$ *s.t.*$$E_{N} \subset (-\frac{1}{4}, \frac{1}{4})$$.
	For any $$j=1, \cdots, n-1$$, let $$k_{l}^{j}$$ be any sequence *s.t.*\\[k_{l}^{j}\alpha_{i}\to \frac{1}{N}\delta_{i, j}, i=1, 2, \cdots, n-1\\]
	Then $$Nk_{l}^{j}(\alpha_{i})\to 0$$, and $$Nk_{l}^{j}\alpha_{n}\to 0$$. Similarly $$(k_{l}^{j}-k_{l+1}^{j})\alpha_{n}\to 0$$.
	Therefore, $$k_{l}^{j}\alpha_{n}\to \frac{m_{j}}{N}$$ for some $$-\frac{N}{2}<m_{j}\leq \frac{N}{2}$$.
	Similarly, if $$k_{l}^{j}\alpha_{i}\to \frac{1}{2N}\delta_{i, j}$$, then $$k_{l}^{j}\alpha_{n}\to \frac{m_{j}}{2N}, \frac{m_{j}}{2N}+\frac{1}{2}$$.
	Since $$\lim k_{l}^{j}\alpha_{n}\in E_{N}\subset (-\frac{1}{4}, \frac{1}{4})$$, one has $$k_{l}^{j}\alpha_{n}\to \frac{m_{j}}{2N}$$.
	By induction on $$t$$, we have $$k_{l}^{j}\alpha_{n}\to \frac{m_{j}}{2^{t}N}$$ when $$k_{l}^{j}\alpha_{i}\to \frac{1}{2^{t}N}\delta_{i, j}$$.
	And
	\\[
	\lim_{k_{l}\alpha_{j}\to \frac{1}{2^{t}N}u_{j}}k_{l}\alpha_{n}=\frac{1}{2^{t}N}\sum u_{j}m_{j}
	\\]
	For $$N_0>N$$ and $$k: k \alpha_{j}\in (-\frac{1}{N}, \frac{1}{N})$$, pick $$\frac{1}{2^{t}N}u_{j} \in U(k\alpha_{j}, \frac{1}{N_0})$$, and $$k_{l}: k_{l}\alpha_{j}\to \frac{1}{2^{t}N}u_{j}$$,
	then
	$$(k_{l}-k)\alpha_{j}\to \frac{1}{2^{t}N}u_{j}-k \alpha_{j}\in U(0, \frac{1}{N_0})$$,
	\\[
	\begin{split}
	d(k \alpha_{n}, \sum km_{j}\alpha_{j})
	&\leq \lim d(k \alpha_{n}, k_{l}\alpha_{n})+d(k_{l}\alpha_{n}, \sum km_{j}\alpha_{j})\cr
	&\leq r(E_{N_0})+\sum \left|m_{j}\right|\left|k \alpha_{j}-\frac{1}{2^{t}N}u_{j}\right|=r(E_{N_0})+\frac{1}{N_0}N^{2}
	\end{split}
	\\]
	Let $$N_0 \to \infty$$, we obtain $$k(\alpha_{n}-\sum m_{j}\alpha_{j})=0$$, and $$\alpha_{i}, i=1, \cdots, n$$ are $$\mathbb Q$$-linearly relative, a contradiction.


> This post is generated by [my unpublished tex-to-kramdown converter](https://github.com/localghost-blog/tex2kramdown).